\clearpage
\section{Inverse Laplace Transformation}

\begin{align}
    \frac{A}{s-p} \quad &\laplace \quad \epsilon(t)Ae^{pt} \\
    \frac{A}{(s-p)^n} \quad &\laplace \quad \epsilon(t)\frac{t^{n-1}}{(n-1)!}Ae^{pt^{n-1}}
\end{align}

\begin{align}
    Ae^{pt} &= Ae^{(p_r+ip_i)t} \\
            &= Ae^{p_r t} e^{i p_i t} \\
            &= (A_r + iA_i)(e^{p_r t}\cos(p_i t) + ie^{p_r t}\sin(p_i t)) \\
            &= A_r e^{p_r t}\cos(p_i t)
                + i A_r e^{p_r t}\sin(p_i t)
                + i A_i e^{p_r t}\cos(p_i t)
                - A_i e^{p_r t}\sin(p_i t) \\
    \Re(Ae^{pt}) &= A_r e^{p_r t}\cos(p_i t) - A_i e^{p_r t}\sin(p_i t) \\
                 &= e^{p_r t}(A_r\cos(p_i t) - A_i\sin(p_i t))
\end{align}
