\subsection{Heaviside Cover-Up Method}

This method only applies to  distinct  roots of the denominator. However, there
is a workaround shown later, making it the method of choice.

\subsubsection{Third Order Example}

\begin{equation}
    T(s) = \frac{b_0 + b_1s + b_2s^2}{(s-p_1)(s-p_2)(s-p_3)}
         = \frac{A_1}{s-p_1} + \frac{A_2}{s-p_2} + \frac{A_3}{s-p_3}
\end{equation}

To determine $A_1$ by the  cover-up  method,  we  mentally  remove  the  factor
$(s-p_1)$ on the left hand side, and set $s=p_1$:

\begin{equation}
    T(s) = \left.\frac{b_0 + b_1s + b_2s^2}{\cancel{(s-p_1)}(s-p_2)(s-p_3)}\right|_{s=p_1}
         = \frac{b_0 + b_1p_1 + b_2p_1^2}{(p_1-p_2)(p_1-p_3)} = A_1
\end{equation}

Similarly, to determine $A_2$, we mentally remove the  factor $(s-p_2)$ and set
$s=p_2$:

\begin{equation}
    T(s) = \left.\frac{b_0 + b_1s + b_2s^2}{(s-p_1)\cancel{(s-p_2)}(s-p_3)}\right|_{s=p_2}
         = \frac{b_0 + b_1p_2 + b_2p_2^2}{(p_2-p_1)(p_2-p_3)} = A_2
\end{equation}

$A_3$ is calculated the same way:

\begin{equation}
    T(s) = \left.\frac{b_0 + b_1s + b_2s^2}{(s-p_1)(s-p_2)\cancel{(s-p_3)}}\right|_{s=p_3}
         = \frac{b_0 + b_1p_2 + b_2p_2^2}{(p_3-p_1)(p_3-p_2)} = A_3
\end{equation}

\subsection{Extension to Multiple Roots}

In the case of repeated roots, the method above will only yield the coefficient
for the most significant power. This can be  fixed  by  first factoring out the
repeated roots, performing the decomposition on  the inner fraction, fractoring
in the roots again, and performing a second decomposition:

\begin{align}
  T(s) &= \frac{b_0 + b_1s}{(s-p_1)^2(s-p_2)} \\
       &= \frac{1}{s-p_1}\left(\frac{b_0 + b_1s}{(s-p_1)(s-p_2)}\right) \\
       &= \frac{1}{s-p_1}\left(\frac{A_1}{s-p_1} + \frac{A_2}{s-p_2}\right) \\
       &= \frac{A_1}{(s-p_1)^2} + \frac{A_2}{(s-p_1)(s-p_2)} \\
       &= \frac{A_1}{(s-p_1)^2} + \frac{A_3}{s-p_1} + \frac{A_4}{s-p_2}
\end{align}

\subsubsection{Example 4}

\begin{align}
    T(s) &= \frac{(s-8)(s-7)(s-5)(s+4)}{(s-1)^4(s+2)} \\
       &= \frac{(s-8)(s-7)(s-5)}{(s-1)^3}
            \left(\frac{s+4}{(s-1)(s+2)}\right) \\
       &= \frac{(s-8)(s-7)(s-5)}{(s-1)^3}
            \left(\frac{A_1}{s-1} + \frac{A_2}{s+2}\right) \\
       &\text{with}\left[\begin{aligned}
           A_1 &= \left.\frac{s+4}{\cancel{(s-1)}(s+2)}\right|_{s=1}
               &= \nicefrac{5}{3} \\
           A_2 &= \left.\frac{s+4}{(s-1)\cancel{(s+2)}}\right|_{s=-2}
               &= \nicefrac{-2}{3}
       \end{aligned}\right. \\
       &= \frac{(s-8)(s-7)(s-5)}{(s-1)^3}\left(\frac{\nicefrac{5}{3}}{s-1}
            + \frac{\nicefrac{-2}{3}}{s+2}\right) \\
       &= \frac{(s-8)(s-7)(s-5)}{(s-1)^2}\left(\frac{\nicefrac{5}{3}}{(s-1)^2}
            + \frac{\nicefrac{-2}{3}}{(s-1)(s+2)}\right) \\
       &= \frac{(s-8)(s-7)(s-5)}{(s-1)^2}\left(\frac{\nicefrac{5}{3}}{(s-1)^2}
            + \frac{A_3}{s-1}
            + \frac{A_4}{s+2}\right) \\
       &\text{with}\left[\begin{aligned}
           A_3 &= \left.\frac{\nicefrac{-2}{3}}{\cancel{(s-1)}(s+2)}\right|_{s=1}
               &= \nicefrac{-2}{9} \\
           A_4 &= \left.\frac{\nicefrac{-2}{3}}{(s-1)\cancel{(s+2)}}\right|_{s=-2}
               &= \nicefrac{2}{9}
       \end{aligned}\right. \\
       &= \frac{(s-8)(s-7)(s-5)}{(s-1)^2}\left(\frac{\nicefrac{5}{3}}{(s-1)^2}
            + \frac{\nicefrac{-2}{9}}{s-1}
            + \frac{\nicefrac{2}{9}}{s+2}\right) \\
       &= \frac{(s-8)(s-7)(s-5)}{s-1}\left(\frac{\nicefrac{5}{3}}{(s-1)^3}
            + \frac{\nicefrac{-2}{9}}{(s-1)^2}
            + \frac{\nicefrac{2}{9}}{(s-1)(s+2)}\right) \\
       &= \frac{(s-8)(s-7)(s-5)}{s-1}\left(\frac{\nicefrac{5}{3}}{(s-1)^3}
            + \frac{\nicefrac{-2}{9}}{(s-1)^2}
            + \frac{A_5}{s-1}
            + \frac{A_6}{s+2}\right) \\
       &\text{with}\left[\begin{aligned}
           A_5 &= \left.\frac{\nicefrac{2}{9}}{\cancel{(s-1)}(s+2)}\right|_{s=1}
               &= \nicefrac{2}{27} \\
           A_6 &= \left.\frac{\nicefrac{2}{9}}{(s-1)\cancel{(s+2)}}\right|_{s=-2}
               &= \nicefrac{-2}{27}
       \end{aligned}\right. \\
       &= \frac{(s-8)(s-7)(s-5)}{s-1}\left(\frac{\nicefrac{5}{3}}{(s-1)^3}
            + \frac{\nicefrac{-2}{9}}{(s-1)^2}
            + \frac{\nicefrac{2}{27}}{s-1}
            + \frac{\nicefrac{-2}{27}}{s+2}\right)
\end{align}

\begin{align}
  T(s) &= (s-8)(s-7)(s-5)\left(\frac{\nicefrac{5}{3}}{(s-1)^4}
            + \frac{\nicefrac{-2}{9}}{(s-1)^3}
            + \frac{\nicefrac{2}{27}}{(s-1)^2}
            + \frac{\nicefrac{-2}{27}}{(s-1)(s+2)}\right) \\
       &= (s-8)(s-7)(s-5)\left(\frac{\nicefrac{5}{3}}{(s-1)^4}
            + \frac{\nicefrac{-2}{9}}{(s-1)^3}
            + \frac{\nicefrac{2}{27}}{(s-1)^2}
            + \frac{A_7}{s-1}
            + \frac{A_8}{s+2}\right) \\
       &\text{with}\left[\begin{aligned}
           A_7 &= \left.\frac{\nicefrac{-2}{27}}{\cancel{(s-1)}(s+2)}\right|_{s=1}
                = \nicefrac{-2}{81} \\
           A_8 &= \left.\frac{\nicefrac{-2}{27}}{(s-1)\cancel{(s+2)}}\right|_{s=-2}
                = \nicefrac{2}{81}
       \end{aligned}\right. \\
       &= (s-8)(s-7)(s-5)\left(\frac{\nicefrac{5}{3}}{(s-1)^4}
            + \frac{\nicefrac{-2}{9}}{(s-1)^3}
            + \frac{\nicefrac{2}{27}}{(s-1)^2}
            + \frac{\nicefrac{-2}{81}}{s-1}
            + \frac{\nicefrac{2}{81}}{s+2}\right) \\
\end{align}

\begin{align}
  T(s) &= \frac{(s-8)(s-7)(s-5)(s+4)}{(s-1)^4(s+2)} \\
       &= \frac{s^4 - 16s^3 + 51s^2 + 244s - 1120}{(s-1)^4(s+2)} \\
       &= \frac{A_1}{(s-1)^4}
          + \frac{A_2}{(s-1)^3}
          + \frac{A_3}{(s-1)^2}
          + \frac{A_4}{s-1}
          + \frac{A_5}{s+2} \\
       &\text{with}\left[\begin{aligned}
           A_1 &= \left.\frac{s^4 - 16s^3 + 51s^2 + 244s - 1120}{\cancel{(s-1)^4}(s+2)}\right|_{s=1}
                = -280 \\
           A_5 &= \left.\frac{s^4 - 16s^3 + 51s^2 + 244s - 1120}{(s-1)^4\cancel{(s+2)}}\right|_{s=-2}
                = \nicefrac{-140}{9}
       \end{aligned}\right. \\
       &\text{with}\left[\begin{aligned}
           A_2 &= \left.\frac{d}{ds}\left(
                    \frac{s^4 - 16s^3 + 51s^2 + 244s - 1120}{s+2}
                  \right)\right|_{s=1} \\
               &= \left.\frac{(4s^3 - 48s^2 + 102s + 244)(s+2) - (s^4 - 16s^3 + 51s^2 + 244s - 1120)}{(s+2)^2}\right|_{s=1} \\
               &= 194 \\
           A_3 &= \left.\frac{d^2}{ds^2}\left(
                    \frac{s^4 - 16s^3 + 51s^2 + 244s - 1120}{s+2}
                  \right)\right|_{s=1} \\
               &= \left.\frac{d}{ds}\left(
                    \frac{3(s^4 - 8s^3 - 15s^2 + 68s + 536)}{(s+2)^2}
                  \right)\right|_{s=1} \\
               \text{this is wrong}\\
               &= \left.\frac{3(4s^3 - 24s^2 - 30s + 68)(s+2)^2}{(s+2)^4}
                - \frac{3(s^4 - 8s^3 - 15s^2 + 68s + 536)(2s+4)}{(s+2)^4}\right|_{s=1}
       \end{aligned}\right. \\
       &= \frac{-280}{(s-1)^4}
          + \frac{A_2}{(s-1)^3}
          + \frac{A_3}{(s-1)^2}
          + \frac{A_4}{s-1}
          + \frac{\nicefrac{-140}{9}}{s+2} \\
\end{align}
